RelationalAlgebra/NF/BCNF_Impl.lean
@@ -17,124 +17,243 @@ lemma find_BCNF_violator_exec_sound {R : List α} {F : Finset (FunctionalDepende
   have h := List.find?_some h
   trivial
 
-def BCNF_decompose_exec_core (R_list : List α) (R_finset : Finset α) (h_R : R_list.toFinset = R_finset) (F : Finset (FunctionalDependency α)) : DecompositionTree R_finset :=
-  match h_find : find_BCNF_violator_exec R_list F with
+def sublist_via_subset (R : List α) (S : Finset α) : List α :=
+  R.filter (λ a => a ∈ S)
+
+lemma sublist_toFinset_eq_subset {R : List α} {R_sub : Finset α} (h_sub : R_sub ⊆ R.toFinset) :
+  (sublist_via_subset R R_sub).toFinset = R_sub := by
+  simp [sublist_via_subset, Finset.filter_mem_eq_inter]
+  trivial
+
+lemma BCNF_exec_step_cover {R X : List α} {F : Finset (FunctionalDependency α)}
+  (h_vlt : is_BCNF_violator X.toFinset R.toFinset F) :
+  have R₁ := sublist_via_subset R (attr_closure_proj F X.toFinset R.toFinset);
+  have R₂ := sublist_via_subset R ((R.toFinset \ attr_closure_proj F X.toFinset R.toFinset) ∪ X.toFinset);
+  R₁.toFinset ∪ R₂.toFinset = R.toFinset := by
+  intro R₁ R₂
+  rw [sublist_toFinset_eq_subset, sublist_toFinset_eq_subset]
+  apply BCNF_step_cover
+  · exact h_vlt
+  · exact HasSSubset.SSubset.subset (R2_subset_R h_vlt)
+  · exact HasSSubset.SSubset.subset (R1_subset_R h_vlt)
+
+def BCNF_decompose_exec (R : List α) (F : Finset (FunctionalDependency α)) : DecompositionTree R.toFinset :=
+  let R_finset := R.toFinset
+  have h_R : R.toFinset = R_finset := by dsimp
+  match h_find : find_BCNF_violator_exec R F with
   | none => .leaf R_finset
   | some X =>
     have h_violator : is_BCNF_violator X.toFinset R_finset F := by
       rw [← h_R]
       exact find_BCNF_violator_exec_sound h_find
-    let R₁_finset := attr_closure_proj F X.toFinset R_finset
-    let R₂_finset := (R_finset \ attr_closure_proj F X.toFinset R_finset) ∪ X.toFinset
-    let R₁_list := R_list.filter (λ a => a ∈ R₁_finset)
-    let R₂_list := R_list.filter (λ a => a ∈ R₂_finset)
-    have h_R₁ : R₁_list.toFinset = R₁_finset := by
-      simp [R₁_list, h_R, Finset.filter_mem_eq_inter]
-      exact attr_closure_proj_subset
-    have h_R₂ : R₂_list.toFinset = R₂_finset := by
-      simp [R₂_list, h_R, Finset.filter_mem_eq_inter]
-      unfold R₂_finset
-      apply Finset.union_subset
-      · simp
-      · simp [is_BCNF_violator] at h_violator
-        exact h_violator.1
-    .node (Decomposition.mk R₁_finset R₂_finset (BCNF_step_cover h_violator))
-          (BCNF_decompose_exec_core R₁_list R₁_finset h_R₁ F)
-          (BCNF_decompose_exec_core R₂_list R₂_finset h_R₂ F)
-termination_by R_finset.card
+    let R₁ := sublist_via_subset R (attr_closure_proj F X.toFinset R_finset)
+    let R₂ := sublist_via_subset R ((R_finset \ attr_closure_proj F X.toFinset R_finset) ∪ X.toFinset)
+    .node (Decomposition.mk R₁.toFinset R₂.toFinset (BCNF_exec_step_cover h_violator))
+          (BCNF_decompose_exec R₁ F)
+          (BCNF_decompose_exec R₂ F)
+termination_by R.toFinset.card
 decreasing_by
-  · exact Finset.card_lt_card (R1_subset_R h_violator)
-  · exact Finset.card_lt_card (R2_subset_R h_violator)
+  · have h := R1_subset_R h_violator
+    rw [← h_R] at h
+    rw [sublist_toFinset_eq_subset (HasSSubset.SSubset.subset h)]
+    exact Finset.card_lt_card h
+  · have h := R2_subset_R h_violator
+    rw [← h_R] at h
+    rw [sublist_toFinset_eq_subset (HasSSubset.SSubset.subset h)]
+    exact Finset.card_lt_card (R2_subset_R h_violator)
 
-def BCNF_decompose_exec (R : List α) (F : Finset (FunctionalDependency α)) : DecompositionTree R.toFinset :=
-  BCNF_decompose_exec_core R R.toFinset (by simp) F
+noncomputable def list_based_picker (Universe : List α) (F : Finset (FunctionalDependency α))
+  (R_finset : Finset α) : Option (Finset α) :=
+  if R_finset ⊆ Universe.toFinset then
+    let R_cur_list := sublist_via_subset Universe R_finset
+    (find_BCNF_violator_exec R_cur_list F).map List.toFinset
+  else
+    let violators := find_BCNF_violators R_finset F
+    if h_no_vlts : violators = ∅ then none
+    else some (Classical.choose (Finset.nonempty_of_ne_empty h_no_vlts))
 
-lemma BCNF_decompose_exec_core_lossless {R_list : List α} {R_finset : Finset α} (h_R : R_list.toFinset = R_finset) {F : Finset (FunctionalDependency α)} :
-  (BCNF_decompose_exec_core R_list R_finset h_R F).is_lossless F := by
-  induction R_list, R_finset, h_R using BCNF_decompose_exec_core.induct F with
-  | case1 _ h_none =>
-    unfold DecompositionTree.is_lossless BCNF_decompose_exec_core
-    split
-    · trivial
-    · next h =>
-      split at h
-      · contradiction
-      · next heq =>
-        rw [h_none] at heq
-        contradiction
-  | case2 _ _ h_find _ R₁_finset R₂_finset R₁_list R₂_list =>
-    next ih₁ ih₂ =>
-    rw [BCNF_decompose_exec_core]
-    split
-    · next h_none =>
-      rw [h_find] at h_none
-      contradiction
-    · next X' h_find' =>
-      rw [DecompositionTree.is_lossless]
-      constructor
-      · apply BCNF_decompose_step_is_lossless
-        apply find_BCNF_violator_exec_sound
-        exact h_find'
-      · simp [h_find'] at h_find
-        subst X'
-        unfold R₁_finset R₁_list at ih₁
-        unfold R₂_finset R₂_list at ih₂
-        exact ⟨ih₁, ih₂⟩
-
-theorem BCNF_decompose_exec_lossless {R : List α} {F : Finset (FunctionalDependency α)} :
-  (BCNF_decompose_exec R F).is_lossless F := by
-  unfold BCNF_decompose_exec
-  apply BCNF_decompose_exec_core_lossless
-
-lemma all_are_BCNF_recursive {R R₁ R₂ : Finset α} {LT : DecompositionTree R₁} {RT : DecompositionTree R₂} {F : Finset (FunctionalDependency α)}
-  (h_cover : R₁ ∪ R₂ = R)
-  (h_LT : all_are_BCNF LT F) (h_RT : all_are_BCNF RT F) :
-  all_are_BCNF (DecompositionTree.node (Decomposition.mk R₁ R₂ h_cover) LT RT) F := by
-  simp_all [all_are_BCNF]
-  intro L h_L
-  rw [DecompositionTree.leaves, Finset.mem_union] at h_L
-  rcases h_L with h_L₁ | h_L₂
-  · exact h_LT h_L₁
-  · exact h_RT h_L₂
-
-lemma BCNF_decompose_exec_core_leaves_are_BCNF {R_list : List α} {R_finset : Finset α} (h_R : R_list.toFinset = R_finset) {F : Finset (FunctionalDependency α)} :
-  all_are_BCNF (BCNF_decompose_exec_core R_list R_finset h_R F) F := by
-  induction R_list, R_finset, h_R using BCNF_decompose_exec_core.induct F with
-  | case1 R_list h_none =>
-    unfold all_are_BCNF BCNF_decompose_exec_core DecompositionTree.leaves
-    simp_all
-    split
-    · simp [BCNF_sem_eq_syn, is_BCNF_syn]
-      simp [find_BCNF_violator_exec] at h_none
-      intro X h_X
-      let x := R_list.filter (λ a => a ∈ X)
-      have h_x : x.toFinset = X := by
-        simp [x, Finset.filter_mem_eq_inter]
-        exact h_X
-      have h_sublist : x.Sublist R_list := by simp [x]
-      apply h_none at h_sublist
-      simp [is_BCNF_violator, h_x] at h_sublist
+lemma no_vlts_equiv {R : List α} {F : Finset (FunctionalDependency α)} :
+  find_BCNF_violator_exec R F = none ↔ find_BCNF_violators R.toFinset F = ∅ := by
+  constructor
+  · intro h_exec_none
+    unfold find_BCNF_violator_exec at h_exec_none
+    rw [Finset.eq_empty_iff_forall_notMem]
+    intro X h_X
+    rw [find_BCNF_violators, Finset.mem_filter, Finset.mem_powerset] at h_X
+    obtain ⟨h_sub, h_violator⟩ := h_X
+    let X_list := R.filter (λ a => a ∈ X)
+    have h_X_list_sublist : X_list.Sublist R := List.filter_sublist
+    have h_mem_sublists : X_list ∈ R.sublists := List.mem_sublists.mpr h_X_list_sublist
+    have h_X_list_eq : X_list.toFinset = X := sublist_toFinset_eq_subset h_sub
+    have h_not_violator_bool := List.find?_eq_none.mp h_exec_none X_list h_mem_sublists
+    have h_not_violator : ¬ is_BCNF_violator X_list.toFinset R.toFinset F := by
+      apply of_decide_eq_false
+      simp_all
+    rw [h_X_list_eq] at h_not_violator
+    contradiction
+  · intro h_no_vlts
+    simp [find_BCNF_violators, Finset.eq_empty_iff_forall_notMem] at h_no_vlts
+    apply List.find?_eq_none.mpr
+    intro X h_mem_sublists
+    have h_sub : X.toFinset ⊆ R.toFinset := by
+      rw [List.mem_sublists] at h_mem_sublists
+      have h_sub' := h_mem_sublists.subset
+      intro a ha
+      simp_all [List.mem_toFinset]
       tauto
-    · next h =>
-      split at h
-      · contradiction
-      · next h_find =>
+    simp_all
+
+lemma list_based_picker_valid (Universe : List α) (F : Finset (FunctionalDependency α)):
+  is_picker_valid F (list_based_picker Universe F) := by
+  unfold is_picker_valid list_based_picker
+  intro R_finset
+  dsimp only
+  split
+  · next h_sub =>
+    let R_list := sublist_via_subset Universe R_finset
+    have h_R : R_list.toFinset = R_finset := by
+      rw [sublist_toFinset_eq_subset h_sub]
+    match h_find : find_BCNF_violator_exec R_list F with
+    | none =>
+      left
+      rw [← h_R, ← no_vlts_equiv]
+      trivial
+    | some X_list =>
+      right
+      constructor
+      · exact ⟨X_list.toFinset, rfl⟩
+      · intro X h_eq
+        simp only [Option.map_some, Option.some.injEq] at h_eq
+        subst X
+        have h_violator := find_BCNF_violator_exec_sound h_find
+        simp only [find_BCNF_violators, Finset.mem_filter, Finset.mem_powerset]
+        rw [h_R] at h_violator
+        exact ⟨h_violator.1, h_violator⟩
+  · next h_not_sub =>
+    split
+    · next h_empty =>
+      left
+      exact h_empty
+    · next h_not_empty =>
+      right
+      have h_nonempty : (find_BCNF_violators R_finset F).Nonempty := Finset.nonempty_of_ne_empty h_not_empty
+      constructor
+      · exact ⟨Classical.choose h_nonempty, rfl⟩
+      · intro X h_eq
+        simp only [Option.some.injEq] at h_eq
+        subst X
+        exact Classical.choose_spec h_nonempty
+
+lemma filter_subset_eq_filter {α : Type} [DecidableEq α] (L : List α) {S₁ S₂ : Finset α} (h_sub : S₂ ⊆ S₁) :
+  (L.filter (λ a => a ∈ S₁)).filter (λ a => a ∈ S₂) = L.filter (λ a => a ∈ S₂) := by
+  induction L with
+  | nil => rfl
+  | cons hd tl ih =>
+    by_cases h2 : hd ∈ S₂
+    · have h1 : hd ∈ S₁ := h_sub h2
+      simp [h1, h2, ih]
+    · by_cases h1 : hd ∈ S₁
+      · simp [h1, h2, ih]
+      · simp [h1, h2, ih]
+
+lemma sublist_eq_filter_toFinset {Universe R : List α}
+  (h_eq : R = sublist_via_subset Universe R.toFinset)
+  {S : Finset α} (hS : S ⊆ R.toFinset) :
+  sublist_via_subset R S = sublist_via_subset Universe (sublist_via_subset R S).toFinset := by
+  have h_finset : (sublist_via_subset R S).toFinset = S := sublist_toFinset_eq_subset hS
+  rw [h_finset]
+  calc sublist_via_subset R S
+    _ = (Universe.filter (λ a => a ∈ R.toFinset)).filter (λ a => a ∈ S) := by
+      unfold sublist_via_subset at *
+      rw [← h_eq]
+    _ = Universe.filter (λ a => a ∈ S) := filter_subset_eq_filter Universe hS
+    _ = sublist_via_subset Universe S := by rfl
+
+lemma BCNF_decompose_equiv_core {F : Finset (FunctionalDependency α)}
+  (Universe R : List α) (h_sub : R.toFinset ⊆ Universe.toFinset)
+  (h_eq : R = sublist_via_subset Universe R.toFinset) :
+  let picker := list_based_picker Universe F;
+  BCNF_decompose_exec R F = BCNF_decompose R.toFinset F picker := by
+  intro picker
+  induction R using BCNF_decompose_exec.induct F with
+  | case1 R R_finset h_R h_none =>
+    have h_exec : BCNF_decompose_exec R F = .leaf R.toFinset := by
+      unfold BCNF_decompose_exec
+      dsimp
+      split
+      · rfl
+      · next X h_find =>
         rw [h_none] at h_find
         contradiction
-  | case2 _ _ h_find h_violator R₁_finset R₂_finset R₁_list R₂_list =>
-    next ih₁ ih₂ =>
-    unfold BCNF_decompose_exec_core
-    split
-    · next h_none =>
-      rw [h_find] at h_none
-      contradiction
-    · next X' h_find' =>
-      simp [h_find'] at h_find
-      subst X'
-      apply all_are_BCNF_recursive (h_cover := BCNF_step_cover h_violator)
-      · unfold R₁_finset R₁_list at ih₁
-        exact ih₁
-      · unfold R₂_finset R₂_list at ih₂
-        exact ih₂
+    have h_thry : BCNF_decompose R.toFinset F picker = .leaf R.toFinset := by
+      rw [no_vlts_equiv] at h_none
+      unfold BCNF_decompose
+      simp [h_none]
+    rw [h_exec, h_thry]
+  | case2 R R_finset h_R X h_find h_violator R₁ R₂ _ => next ih₁ ih₂ =>
+    subst R_finset
+    have h_exec : BCNF_decompose_exec R F =
+      .node (Decomposition.mk R₁.toFinset R₂.toFinset (BCNF_exec_step_cover h_violator))
+      (BCNF_decompose_exec R₁ F) (BCNF_decompose_exec R₂ F) := by
+      rw [BCNF_decompose_exec]
+      dsimp
+      split
+      · next h =>
+        rw [h_find] at h
+        contradiction
+      · next X' h_find' =>
+        simp [h_find] at h_find'
+        subst X' R₁ R₂
+        rfl
+    have h_R₁ := HasSSubset.SSubset.subset (R1_subset_R h_violator)
+    have h_R₂ := HasSSubset.SSubset.subset (R2_subset_R h_violator)
+    have h_thry : BCNF_decompose R.toFinset F picker =
+      .node (Decomposition.mk R₁.toFinset R₂.toFinset (BCNF_exec_step_cover h_violator))
+      (BCNF_decompose R₁.toFinset F picker) (BCNF_decompose R₂.toFinset F picker) := by
+      rw [BCNF_decompose]
+      split
+      · next h_vlts_empty =>
+        rw [← no_vlts_equiv, h_find] at h_vlts_empty
+        contradiction
+      · next h_vlts =>
+        have h_valid_vlt := (list_based_picker_valid Universe F).resolve_left h_vlts
+        have h_picker : picker R.toFinset = some X.toFinset := by
+          unfold picker list_based_picker
+          simp [h_sub, ← h_eq, h_find]
+        simp [h_picker, h_valid_vlt.2 h_picker]
+        rw [sublist_toFinset_eq_subset h_R₁, sublist_toFinset_eq_subset h_R₂]
+        trivial
+    have h_R₁_sub_univ : R₁.toFinset ⊆ Universe.toFinset := by
+      rw [sublist_toFinset_eq_subset h_R₁]
+      exact Finset.Subset.trans h_R₁ h_sub
+    have h_R₂_sub_univ : R₂.toFinset ⊆ Universe.toFinset := by
+      rw [sublist_toFinset_eq_subset h_R₂]
+      exact Finset.Subset.trans h_R₂ h_sub
+    have h_R₁_eq_univ := sublist_eq_filter_toFinset h_eq h_R₁
+    have h_R₂_eq_univ := sublist_eq_filter_toFinset h_eq h_R₂
+    rw [h_exec, h_thry, ih₁ h_R₁_sub_univ h_R₁_eq_univ, ih₂ h_R₂_sub_univ h_R₂_eq_univ]
+
+theorem BCNF_decompose_equiv
+  {F : Finset (FunctionalDependency α)} {R : List α} :
+  BCNF_decompose_exec R F = BCNF_decompose R.toFinset F (list_based_picker R F) := by
+  apply BCNF_decompose_equiv_core R
+  · exact Finset.Subset.refl _
+  · unfold sublist_via_subset
+    symm
+    apply List.filter_eq_self.mpr
+    intro a ha
+    simp_all
+
+theorem BCNF_decompose_exec_is_lossless {R : List α} {F : Finset (FunctionalDependency α)}
+  : (BCNF_decompose_exec R F).is_lossless F := by
+  rw [BCNF_decompose_equiv]
+  apply BCNF_decompose_is_lossless
+  exact list_based_picker_valid R F
+
+theorem BCNF_decompose_exec_leaves_are_BCNF {R : List α} {F : Finset (FunctionalDependency α)} :
+  all_are_BCNF (BCNF_decompose_exec R F) F := by
+  rw [BCNF_decompose_equiv]
+  apply BCNF_decompose_leaves_are_BCNF
+  exact list_based_picker_valid R F
 
 end RM.NF
